{
 "cells": [
  {
   "cell_type": "markdown",
   "id": "8261c513f42efbd8",
   "metadata": {
    "collapsed": true,
    "jupyter": {
     "outputs_hidden": true
    }
   },
   "source": [
    "# Exercise Sheet 01\n",
    "Tomy Huy Le - 7021280\n",
    "Bachelor Wirtschaftsinformatik\n",
    "\n",
    "This submission is a Python Jupyter notebook containing the solutions for the exercises. There will be Python code cells that can be executed to test my pseudocode solutions and verify their correctness. In addition Markdown cells will be used to explain my solutions and help with formatting."
   ]
  },
  {
   "cell_type": "markdown",
   "id": "c264fa23f3d5413a",
   "metadata": {},
   "source": [
    "## Exercise 1"
   ]
  },
  {
   "cell_type": "markdown",
   "id": "8ad83d636cde52a0",
   "metadata": {},
   "source": [
    "### a)\n",
    "The algorithm `ALG1` first **sorts** the array `A` and then **iterates** through it to find a discrepancy between the array indices and the values they contain. The core idea is that if no number were missing, a sorted array `A` (using 1-based indexing) of numbers from `{0, ..., n}` would have the property that `A[i] = i-1` for all `i` from `1` to `n`. The missing number `x` creates a \"shift\" in this pattern due to the offset of indices and array values.\n",
    "\n",
    "To prove the algorithm is correct, we must show it works for all possible values of the missing number `x`. We can split this into two cases.\n",
    "\n",
    "---\n",
    "\n",
    "#### Case 1: The missing number `x` is less than `n` ($0 \\le x < n$)\n",
    "\n",
    "1.  **Array State after Sorting**:\n",
    "    After sorting, the array `A` will contain all numbers from `{0, ..., n}` except `x`, in ascending order.\n",
    "    The contents of `A` will be:\n",
    "    $$A = [0, 1, 2, \\dots, x-1, x+1, \\dots, n]$$\n",
    "    Using 1-based indexing as in the pseudocode, we have:\n",
    "    - For indices `i` from `1` to `x`:  `A[i] = i-1` as we stated.\n",
    "    - At index `i = x+1`: The value is `A[x+1] = x+1`,  because the missing number disrupts the pattern of `A[i] = i-1`.\n",
    "\n",
    "2.  **Loop Execution**:\n",
    "    The algorithm iterates from `i=1` to `n`.\n",
    "    -   **For `i` from `1` to `x`**: The condition `if A[i] == i` is checked. Since `A[i] = i-1` in this range, the check becomes `if i-1 == i`, which is **false** and the loop continues.\n",
    "    -   **At `i = x+1`**: The condition `if A[i] == i` is checked. At this index, `A[x+1] = x+1`. The check becomes `if x+1 == x+1`, which is **true** because of the missing number.\n",
    "\n",
    "3.  **Return Value**:\n",
    "    The condition is met for the first time at `i = x+1`. The procedure then executes `return i-1`.\n",
    "    $$\\text{return} \\ (x+1) - 1 = x$$\n",
    "    This is the correct missing number.\n",
    "\n",
    "---\n",
    "\n",
    "#### Case 2: The missing number `x` is `n`\n",
    "\n",
    "1.  **Array State after Sorting**:\n",
    "    If `x=n` is missing, the array `A` contains all numbers from `0` to `n-1`. After sorting, `A` will be:\n",
    "    $$A = [0, 1, 2, \\dots, n-1]$$\n",
    "    Using 1-based indexing, this means that for every index `i` from `1` to `n`, the property `A[i] = i-1` holds true.\n",
    "\n",
    "2.  **Loop Execution**:\n",
    "    The algorithm iterates from `i=1` to `n`. At each step, it checks the condition `if A[i] == i`.\n",
    "    - Since `A[i] = i-1` for all `i` in the loop, the check is always `if i-1 == i`, which is always **false**.\n",
    "\n",
    "3.  **Return Value**:\n",
    "    The `if` condition is never satisfied. The loop completes without returning. The procedure then moves to the final line, which is `return n`. This is the correct missing number, `x=n`.\n",
    "\n",
    "---\n",
    "\n",
    "#### Conclusion\n",
    "\n",
    "Since the algorithm correctly computes the missing number `x` in all possible cases (`x < n` and `x = n`) and it is guaranteed that the array contains exactly one number from 0..n with one missing number the algorithm is **correct**."
   ]
  },
  {
   "cell_type": "markdown",
   "id": "1299941c936197a6",
   "metadata": {},
   "source": [
    "### b)\n",
    "### Proof of Correctness for ALG2\n",
    "\n",
    "The algorithm `ALG2` finds the difference between an expected sum and an actual sum. The set of numbers *should* be `{0, 1, ..., n}` with 'n' as the length of the array which we know. But the array `A` is missing one number, `x`. The algorithm calculates the sum of all numbers in the incomplete array `A` and subtracts it from the sum of a known, complete sequence of numbers (the sum of the numbers from 0 to n).\n",
    "\n",
    "To prove the algorithm is correct, we need to proof that the algorithm correctly calculates the difference between the two sums.\n",
    "\n",
    "---\n",
    "### 1. The two sums\n",
    "\n",
    "* Let `S_full` be the sum of all numbers in the complete set `{0, 1, ..., n}`.\n",
    "    $$S_{full} = \\sum_{k=0}^{n} k$$\n",
    "\n",
    "* Let `S_A` be the sum of all the numbers actually present in the input array `A`. Since `A` contains `n` elements, this sum is:\n",
    "    $$S_A = \\sum_{i=1}^{n} A[i]$$\n",
    "\n",
    "#### 2. The Key Relationship\n",
    "\n",
    "The set of numbers in array `A` is the same as the complete set `{0, 1, ..., n}` but with the number `x` removed. Therefore, the sum of `A`'s elements (`S_A`) is simply the sum of the full set (`S_full`) minus the missing number `x`.\n",
    "\n",
    "$$S_A = S_{full} - x$$\n",
    "\n",
    "Substituting the definition of `S_full`, we get:\n",
    "\n",
    "$$S_A = \\left(\\sum_{k=0}^{n} k\\right) - x$$\n",
    "\n",
    "---\n",
    "\n",
    "#### 3. Analyzing the Algorithm's Calculation\n",
    "\n",
    "The algorithm initializes a variable `y` to 0 and then iterates from `i=1` to `n`. In each step, it calculates `y = y + i - A[i]`. Let's analyze the final value of `y` after the loop has finished.\n",
    "\n",
    "The final value is the sum of all the `i` values minus the sum of all the `A[i]` values:\n",
    "\n",
    "$$y = \\sum_{i=1}^{n} (i - A[i])$$\n",
    "\n",
    "Using the properties of summation, we can split this into two separate sums:\n",
    "\n",
    "$$y = \\left(\\sum_{i=1}^{n} i\\right) - \\left(\\sum_{i=1}^{n} A[i]\\right)$$\n",
    "\n",
    "We recognize the second term as `S_A`. So:\n",
    "\n",
    "$$y = \\left(\\sum_{i=1}^{n} i\\right) - S_A$$\n",
    "\n",
    "---\n",
    "\n",
    "#### 4. Final Derivation\n",
    "\n",
    "Now, we substitute our expression for `S_A` from step 2 into the equation for `y`:\n",
    "\n",
    "$$y = \\left(\\sum_{i=1}^{n} i\\right) - \\left[ \\left(\\sum_{k=0}^{n} k\\right) - x \\right]$$\n",
    "\n",
    "To simplify, let's expand the sum from `k=0` to `n`:\n",
    "\n",
    "$$\\sum_{k=0}^{n} k = 0 + \\sum_{k=1}^{n} k = \\sum_{i=1}^{n} i$$\n",
    "\n",
    "(Note that the index variable `k` or `i` doesn't matter, the sum is the same).\n",
    "\n",
    "Now substitute this back into the equation for `y`:\n",
    "\n",
    "$$y = \\left(\\sum_{i=1}^{n} i\\right) - \\left[ \\left(\\sum_{i=1}^{n} i\\right) - x \\right]$$\n",
    "\n",
    "Distributing the negative sign gives:\n",
    "\n",
    "$$y = \\left(\\sum_{i=1}^{n} i\\right) - \\left(\\sum_{i=1}^{n} i\\right) + x$$\n",
    "\n",
    "The two summations cancel each other out, leaving:\n",
    "\n",
    "$$y = x$$\n",
    "\n",
    "---\n",
    "\n",
    "#### Conclusion\n",
    "\n",
    "The final value of `y` returned by the algorithm is exactly equal to the missing number `x`. Therefore, the algorithm is **correct**."
   ]
  },
  {
   "cell_type": "markdown",
   "id": "af29256f7ca54c47",
   "metadata": {},
   "source": [
    "## Exercise 2"
   ]
  },
  {
   "cell_type": "markdown",
   "id": "f76523361cae280",
   "metadata": {},
   "source": [
    "Before we can start with the correction proof we have to take a look at the definition of the polynomial.\n",
    "\n",
    "$$p(X) = \\sum_{i=0}^{n} a_i \\cdot X^i = a_0 + a_1 \\cdot X^1 + a_2 \\cdot X^2 + a_3 \\cdot X^3 + \\dots + a_{n-1} \\cdot X^{n-1} + a_n \\cdot X^n$$\n",
    "\n",
    "This can be further simplified into:\n",
    "\n",
    "$$a_0 + X(a_1 + X(a_2 + X(a_3 + \\dots + X(a_{n-1} + X \\cdot a_n))))$$\n",
    "\n",
    "### Correction Proof\n",
    "\n",
    "First we set $y$ to 0 and start our `for` loop starting with $n$ and moving backwards to 0. Inside the loop we then have the calculation $y = a_i + z \\cdot y$. Through the iterative process of the calculation we know $y$ is our accumulator throughout this process. If we would now start this process we would get this:\n",
    "\n",
    "-   $y = a_n + z \\cdot 0$\n",
    "-   $y = a_{n-1} + z \\cdot a_n$\n",
    "-   $y = a_{n-2} + z \\cdot (a_{n-1} + z \\cdot a_n)$\n",
    "-   ... _we do this until y = a_0 + z(a_1 + z(...))_\n",
    "\n",
    "As one can see we are slowly getting the formula of the polynomial we have discussed earlier before the correction proof.\n",
    "\n",
    "By repeating the process of scaling the polynomial with $z$ from the previous iteration and adding the next coefficient, we ensure the correct accumulation of $a_i$ for every $i \\in \\{0, \\dots, n\\}$ in $y$. After our loop we return our accumulator $y$, which through the previous explanation gives us exactly the polynomial $p(z)$."
   ]
  },
  {
   "cell_type": "markdown",
   "id": "41ad4ba03af2afcc",
   "metadata": {},
   "source": [
    "## Exercise 3"
   ]
  },
  {
   "cell_type": "markdown",
   "id": "42f2c3269cfc97d5",
   "metadata": {},
   "source": [
    "By definition from the lecture we know that if $f \\in O(g)$ holds:\n",
    "$$O(g) := \\{f \\ge 0 \\mid \\exists c > 0: f \\le_{ae} c \\cdot g\\}$$\n",
    "\n",
    "---\n",
    "#### a. Additivity Proof:\n",
    "\n",
    "$f_1 = O(g_1)$ and $f_2 = O(g_2)$ | combine both\n",
    "\n",
    "$f_1 + f_2 = O(g_1) + O(g_2)$ | use of definition from the lecture\n",
    "\n",
    "$f_1 + f_2 \\le_{ae} c_1 \\cdot g_1 + c_2 \\cdot g_2$ | combine both c's into one, since they are both constants\n",
    "\n",
    "$f_1 + f_2 \\le_{ae} c_3 \\cdot (g_1 + g_2)$ | use of definition from the lecture\n",
    "\n",
    "$f_1 + f_2 = O(g_1 + g_2)$\n",
    "\n",
    "if $g_1 > g_2$ then we get $f_1 + f_2 = O(g_1)$\n",
    "\n",
    "if $g_1 < g_2$ then we get $f_1 + f_2 = O(g_2)$\n",
    "\n",
    "Therefore $f_1 + f_2$ is bounded by $O(\\max(g_1, g_2))$\n",
    "\n",
    "To determine which one of these is the max, we use the max function\n",
    "\n",
    "$f_1 + f_2 = O(\\max(g_1, g_2))$\n",
    "\n",
    "---\n",
    "#### b. Multiplicativity Proof:\n",
    "\n",
    "$f_1 = O(g_1)$ and $f_2 = O(g_2)$ | combine both\n",
    "\n",
    "$f_1 \\cdot f_2 = O(g_1) \\cdot O(g_2)$ | use of definition from the lecture\n",
    "\n",
    "$f_1 \\cdot f_2 \\le_{ae} c_1 \\cdot g_1 \\cdot c_2 \\cdot g_2$ | combine both c's into one, since they are both constants\n",
    "\n",
    "$f_1 \\cdot f_2 \\le_{ae} c_3 \\cdot (g_1 \\cdot g_2)$ | use of definition from the lecture\n",
    "\n",
    "$f_1 \\cdot f_2 = O(g_1 \\cdot g_2)$\n",
    "\n",
    "---\n",
    "#### c. Transitivity Proof\n",
    "\n",
    "$f = O(g)$ | use definition from lecture\n",
    "\n",
    "$f = c \\cdot g$ | use definition from exercise\n",
    "\n",
    "$f = c \\cdot O(h)$ | use definition of O - Notation for constants\n",
    "\n",
    "$f = O(h)$\n",
    "\n",
    "---\n",
    "#### d.\n",
    "\n",
    "We need to prove that for any $k > 0$, we have $f^c \\le_{ae} k \\cdot b^f$.\n",
    "\n",
    "Since $f = \\omega(1)$, there is an $n_0$ such that for all $n \\ge n_0$, we have $\\sqrt{f(n)} \\ge \\max(1, -\\ln k, \\frac{c+1}{\\ln b})$.\n",
    "\n",
    "This gives us the inequality:\n",
    "$$-\\ln k \\le \\sqrt{f(n)}$$\n",
    "\n",
    "Which we can expand to:\n",
    "$$-\\ln k \\le \\sqrt{f(n)}(\\sqrt{f(n)}\\ln b - c) = f(n)\\ln b - c\\sqrt{f(n)}$$\n",
    "\n",
    "Rearranging yields:\n",
    "$$c\\sqrt{f(n)} \\le f(n)\\ln b + \\ln k$$\n",
    "\n",
    "From the inequality $\\ln(1+x) \\le \\frac{x}{\\sqrt{1+x}}$, we can show that $c \\ln f(n) \\le c\\sqrt{f(n)}$. This leads to:\n",
    "$$c \\ln f(n) \\le f(n)\\ln b + \\ln k$$\n",
    "\n",
    "Exponentiating both sides gives:\n",
    "$$e^{c \\ln f(n)} = f(n)^c \\le e^{f(n) \\ln b + \\ln k} = e^{f(n) \\ln b} \\cdot e^{\\ln k} = b^{f(n)} \\cdot k$$\n",
    "\n",
    "Therefore, we have shown:\n",
    "$$f^c \\le_{ae} k \\cdot b^f$$"
   ]
  },
  {
   "cell_type": "markdown",
   "id": "907a634474bd4877",
   "metadata": {},
   "source": [
    "## Exercise 4\n",
    "\n",
    "First we can simplify the functions, by using Big O-Notation, since we can ignore constant factors for large n.\n",
    "\n",
    "-   $2n^2 - 4n \\rightarrow O(n^2)$\n",
    "-   $n^2 \\log n \\rightarrow O(n^2 \\log n)$\n",
    "-   $n \\log n \\rightarrow O(n \\log n)$\n",
    "-   $2^n \\rightarrow O(2^n)$\n",
    "-   $\\log n \\rightarrow O(\\log n)$\n",
    "-   $n \\log(\\log n) \\rightarrow O(n \\log(\\log n))$\n",
    "\n",
    "Considering the law of transitivity from exercise 3b, the final ordering from slowest to fastest asymptotic growth is:\n",
    "\n",
    "$$\\log n < n \\log \\log n < n \\log n < 2n^2 - 4n < n^2 \\log n < 2^n$$\n",
    "\n",
    "Proofs by considering the mathematical asymptotic behavior:\n",
    "\n",
    "**Proof for $\\log n \\in o(n \\log \\log n)$**\n",
    "\n",
    "$$\\lim_{n \\to \\infty} \\frac{\\log n}{n \\log \\log n} = \\lim_{n \\to \\infty} \\frac{\\log n}{n} \\cdot \\frac{1}{\\log \\log n} = 0$$\n",
    "\n",
    "**Proof for $$\\lim_{n \\to \\infty} \\frac{\\log n}{n}$$**\n",
    "\n",
    "$$= \\lim_{n \\to \\infty} \\frac{1/n}{1} \\quad (L'Hôpital)$$\n",
    "\n",
    "$$= \\lim_{n \\to \\infty} \\frac{1}{n} = 0$$\n",
    "(This holds because both $\\frac{\\log n}{n}$ and $\\frac{1}{\\log \\log n}$ move towards 0 as $n \\to \\infty$)\n",
    "\n",
    "---\n",
    "\n",
    "**Proof for $n \\log \\log n \\in o(n \\log n)$**\n",
    "\n",
    "$$\\lim_{n \\to \\infty} \\frac{n \\log \\log n}{n \\log n} = \\lim_{n \\to \\infty} \\frac{\\log \\log n}{\\log n}$$\n",
    "\n",
    "Using L'Hôpital's Rule:\n",
    "\n",
    "$$= \\lim_{n \\to \\infty} \\frac{\\frac{d}{dn}(\\log \\log n)}{\\frac{d}{dn}(\\log n)} = \\lim_{n \\to \\infty} \\frac{\\frac{1}{n \\log n}}{\\frac{1}{n}} = \\lim_{n \\to \\infty} \\frac{n}{n \\log n} = \\lim_{n \\to \\infty} \\frac{1}{\\log n} = 0$$\n",
    "\n",
    "---\n",
    "\n",
    "**Proof for $n \\log n \\in o(2n^2 - 4n)$**\n",
    "\n",
    "$$\\lim_{n \\to \\infty} \\frac{n \\log n}{2n^2 - 4n} = \\lim_{n \\to \\infty} \\frac{n \\log n}{n \\cdot (2n - 4)} = \\lim_{n \\to \\infty} \\frac{\\log n}{2n - 4}$$\n",
    "\n",
    "Using L'Hôpital's Rule:\n",
    "\n",
    "$$= \\lim_{n \\to \\infty} \\frac{1/n}{2} = 0$$\n",
    "\n",
    "---\n",
    "\n",
    "**Proof for $2n^2 - 4n \\in o(n^2 \\log n)$**\n",
    "\n",
    "$$\\lim_{n \\to \\infty} \\frac{2n^2 - 4n}{n^2 \\log n} = \\lim_{n \\to \\infty} \\frac{n \\cdot (2n - 4)}{n^2 \\log n} = \\lim_{n \\to \\infty} \\frac{2n - 4}{n \\log n}$$\n",
    "\n",
    "Using L'Hôpital's Rule:\n",
    "\n",
    "$$= \\lim_{n \\to \\infty} \\frac{2}{\\log n + 1} = 0$$\n",
    "\n",
    "---\n",
    "\n",
    "#### Proof for $n^2 \\log n \\in o(2^n)$\n",
    "\n",
    "$$\\lim_{n \\to \\infty} \\frac{n^2 \\log n}{2^n}$$\n",
    "\n",
    "$$= \\lim_{n \\to \\infty} \\frac{2n \\log n + n}{2^n \\ln 2} \\quad (L'Hôpital)$$\n",
    "\n",
    "$$= \\lim_{n \\to \\infty} \\frac{2 \\log n + 3}{2^n (\\ln 2)^2} \\quad (L'Hôpital)$$\n",
    "\n",
    "$$= \\lim_{n \\to \\infty} \\frac{2/n}{2^n (\\ln 2)^3} \\quad (L'Hôpital)$$\n",
    "\n",
    "$$= \\lim_{n \\to \\infty} \\frac{2}{n \\cdot 2^n (\\ln 2)^3} = 0$$"
   ]
  }
 ],
 "metadata": {
  "kernelspec": {
   "display_name": "Python 3 (ipykernel)",
   "language": "python",
   "name": "python3"
  },
  "language_info": {
   "codemirror_mode": {
    "name": "ipython",
    "version": 3
   },
   "file_extension": ".py",
   "mimetype": "text/x-python",
   "name": "python",
   "nbconvert_exporter": "python",
   "pygments_lexer": "ipython3",
   "version": "3.13.0"
  }
 },
 "nbformat": 4,
 "nbformat_minor": 5
}
